new/proof/asyncfile.v
@@ -240,25 +240,8 @@ Proof.
   wp_pures.
   wp_load.
   wp_pures.
-  wp_bind (load_ty _ _).
-  eapply (tac_wp_load_ty []).
-  { tc_solve. }
-  { iAssumptionCore. }
+  wp_load.
   wp_pures.
-  (*
-  wp_apply (wp_load_ty with "[$]").
-  {
-    iFrame.
-    eapply coq_tactics.tac_frame with "Hclosed" _ _ _.
-    { done. }
-    { apply _.
-      Print Hint.
-    Disable Notation "↦s[" (all).
-    Set Printing Implicit.
-    Print Hint.
-    Set Typeclasses Debug Verbosity 2.
-    (* FIXME: tc search hangs *) *)
-  simpl.
   wp_pures.
   wp_load.
   wp_pures.
@@ -266,126 +249,6 @@ Proof.
   { (* case: wait *)
     simpl. rewrite decide_True //.
     wp_pures. wp_load. wp_pures.
-    wp_bind (load_ty _ _).
-    Typeclasses Opaque asyncfile.is_defined.
-    Typeclasses Opaque sync.is_defined.
-
-    iRevert "HdurableIndexCond HindexCond".
-    iClear "# ∗".
-    iIntros "HdurableIndexCond Hcond".
-    eapply (tac_wp_load_ty []).
-    { apply _. }
-    {
-
-
-      Check (eq_refl : (struct.field_offset asyncfile.AsyncFile "indexCond"%go) =
-        (struct.field_offset asyncfile.AsyncFile "durableIndexCond"%go)).
-      Eval simpl in (struct.field_offset asyncfile.AsyncFile "indexCond"%go).
-      Transparent w8_word_instance.
-      Eval simpl in (w8_word_instance.(word.add)). (W8 0) (W8 10)).
-      Eval simpl in (word.add (W8 0) (W8 10)).
-      Check w8_word_instance.(word.eqb).
-
-      (* FIXME: making this transparent allows reduction to finish. *)
-      eunify (struct.field_offset asyncfile.AsyncFile "indexCond"%go)
-        (struct.field_offset asyncfile.AsyncFile "durableIndexCond"%go).
-
-(struct.field_offset t f0)
-
-      (* this unify operation runs in iAssumptionCore and gets stuck. *)
-      eunify (struct.field_ref_f asyncfile.AsyncFile "indexCond"%go f)
-              (* ), indexCond) *)
-        (struct.field_ref_f asyncfile.AsyncFile "durableIndexCond"%go f)., _ : loc).
-      eunify
-        (f ↦s[asyncfile.AsyncFile :: "indexCond"%go] indexCond)%I
-        (f ↦s[asyncfile.AsyncFile :: "durableIndexCond"%go] (_ : loc))%I.
-
-
-      Set Ltac Debug.
-
-      Disable Notation "↦s[" (all).
-      Disable Notation "↦" (all).
-      eunify (@typed_pointsto grove_op grove_model grove_interp Σ heapGS0 loc (@into_val_loc grove_op)
-                (struct.field_ref_f asyncfile.AsyncFile "durableIndexCond" f) _
-                _)
-        (@typed_pointsto grove_op grove_model grove_interp Σ heapGS0 loc (@into_val_loc grove_op)
-           (struct.field_ref_f asyncfile.AsyncFile "indexCond" f) (DfracOwn 1) indexCond).
-
-      eunify (@typed_pointsto grove_op grove_model grove_interp Σ heapGS0 loc (@into_val_loc grove_op)
-                (struct.field_ref_f asyncfile.AsyncFile "durableIndexCond" f) _
-                _)
-        (@typed_pointsto grove_op grove_model grove_interp Σ heapGS0 loc (@into_val_loc grove_op)
-           (struct.field_ref_f asyncfile.AsyncFile "indexCond" f) (DfracOwn 1) indexCond).
-
-      Set Ltac Debug.
-      Disable Notation "↦s[" (all).
-      Disable Notation "↦" (all).
-
-      Set Printing Implicit.
-      iAssumptionCore.
-      Import environments reduction.
-      let rec find Γ i P :=
-        lazymatch Γ with
-        | Esnoc ?Γ ?j ?Q => first [unify P Q; unify i j|find Γ i P]
-        end in
-      match goal with
-      | |- envs_lookup ?i (Envs ?Γp ?Γs _) = Some (_, ?P) =>
-          (* find Γs i P *)
-          lazymatch Γs with
-          | Esnoc ?Γs ?j ?Q => set (y:=Q); set (z:=P)
-              (* first [unify P Q; unify i j|find Γs i P] *)
-          end
-      end.
-      unfold y. unfold z.
-      unify y z.
-      iAssumptionCore.
-
-      ltac_tactics.
-      reduction.pm_reflexivity.
-      iAssumptionCore.
-      instantiate (2:=(DfracOwn 1)).
-      instantiate (1:=durableIndexCond).
-      instantiate (1:=false).
-      instantiate (4:=INamed "HdurableIndexCond").
-      done.
-      simpl.
-      iAssumptionCore. }
-
-    wp_apply (wp_load_ty with "[-]").
-    {
-      iClear "Hghost".
-      iClear "#".
-      iClear "Htok HΦ Hlocal1 Hlocal2 Hlocked".
-      Set Typeclasses Debug.
-      iClear "HclosedCond".
-      iFrame.
-      (* eapply tac_frame with "HdurableIndexCond" _ _ _. *)
-      eapply tac_frame with "Hclosed" _ _ _.
-      { done. }
-      {
-        Print Hint.
-        Disable Notation "↦s[" (all).
-        Set Printing Implicit.
-        Print Hint.
-        Set Typeclasses Debug Verbosity 2.
-        instantiate (3:=(DfracOwn 1)).
-        instantiate (3:=(DfracOwn 1)).
-        apply _.
-        simple apply @class_instances_frame.frame_here.
-        typeclasses eauto 1.
-        tc_solve.
-      }
-      iFrameHyp "Hclosed".
-
-
-(Frame false (f ↦s[asyncfile.AsyncFile :: "closed"] closed)
-                  (f ↦s[asyncfile.AsyncFile :: "durableIndexCond"]{?Goal0} ?Goal1)
-                  ?b) with backtracking
-      iFrame.
-      iFrame "HdurableIndexCond".
-      iClear "Htok HΦ Hlocal1 Hlocal2 Hlocked".
-      iFrame.
-    }
     wp_load.
     wp_apply (wp_Cond__Wait with "[-Htok HΦ Hlocal1 Hlocal2]").
     {
@@ -547,13 +410,15 @@ Proof.
   wp_load.
   wp_pures.
   wp_load.
+  iNamed "Hdef".
   wp_apply (wp_Mutex__Lock with "[$]").
   iIntros "[Hlocked Hown]".
   iNamed "Hown".
   wp_pures. wp_load.
   wp_pures. wp_load.
   wp_pures.
-  wp_apply wp_Mutex__Unlock'.
+  wp_apply (wp_Mutex__Unlock' with "[]").
+  { iClear "Hmu". iNamed "His". iNamed "Hdef". done. }
   iIntros (m_unlock) "Hunlock".
   wp_pures. wp_load. wp_pures. wp_store.
   wp_pures.
